almost done with spec for Share

share1.bpl
@@ -42,8 +42,9 @@ const unique ShareCountP: PredicateTypes;
 //need to write the ShareCount constructor so that
 //we can use new for it
 
-//procedure ShareConstructor() returns sc:Ref;
-//ensures ;
+//constructor for Share
+procedure ConstructShare(this:Ref, dc_:Ref);
+ensures dc[this] == dc_;
 
 procedure PackShareCount(this:Ref);
 requires (packed[dc[this], OKP] && (fracOKP[dc[this]] > 0));
@@ -71,8 +72,39 @@ assert packed[this, ShareCountP];
 assert (fracShareCountP[this] > 0);
 }
 
-//procedure main()
-//{
+procedure main()
+//need to add absolutely all global variables 
+//that are being modified, by this method,
+//or transitively by all methods that are called in 
+//this procedure
+modifies val, dbl, packed, fracOKP, fracShareCountP;
+{
+var dc0 : Ref;
+var share1, share2 : Ref;
+//need to state that dc satisfies the OK predicate
+assume packed[dc0, OKP];
+call ConstructShare(share1, dc0);
 
-//}
+call ConstructShare(share2, dc0);
+
+//this assume is for the dc of share1,
+//to say that we put it in the OK predicate
+
+assume fracOKP[dc[share1]] > 0;
+call PackShareCount(share1);
+packed[share1, ShareCountP] := true;
+assert packed[share1, ShareCountP];
+assert (fracShareCountP[share1] > 0);
+
+call touch(share1);
+
+assume fracOKP[dc[share2]] > 0;
+call PackShareCount(share2);
+packed[share2, ShareCountP] := true;
+
+assert packed[share2, ShareCountP];
+assert (fracShareCountP[share2] > 0);
+call touch(share2);
+
+}
 
